Introduce RContext/REngine

src/Solver/RSolver.dfy
@@ -1,30 +1,33 @@
+/// Module RSolver provides three types:
+///   * REXpr - an AST for the solver's expressions
+///   * RContext - a conjunction of assumptions, represented as a node in a tree
+///   * REngine - an SMT-backed engine that can answer proof queries in a given context
 module RSolvers {
   import SolverExpr
   import Solvers
   import Z3SmtSolver
+  import opened Std.Wrappers
 
   export
+    reveals RExpr
+    provides RExpr.Eq
+    provides RContext, CreateEmptyContext
+    reveals REngine
+    provides CreateEngine, REngine.Repr, REngine.Valid, REngine.Prove
+    // ...
     provides RSolver, RSolver.Repr, RSolver.Valid
     provides Create
     provides RSolver.Extend, RSolver.Prove, RSolver.Record
-    reveals RExpr
-    provides RExpr.Eq
     provides SolverExpr, Solvers
 
-  method Create() returns (r: RSolver)
-    ensures r.Valid() && fresh(r.Repr)
-  {
-    var smtEngine := Z3SmtSolver.CreateZ3SolverEngine();
-    var state := new Solvers.SolverState(smtEngine);
-    var solver := Solvers.Solver.Empty();
-    return RSolver(solver, state);
-  }
+  // ===== RExpr =====
 
   datatype RExpr =
     | Boolean(b: bool)
     | Integer(x: int)
     | Id(v: SolverExpr.SVar)
-    | FuncAppl(op: string, args: seq<RExpr>)  {
+    | FuncAppl(op: string, args: seq<RExpr>)
+  {
     function ToSExpr(): SolverExpr.SExpr {
       match this
       case Boolean(b) => SolverExpr.SExpr.Boolean(b)
@@ -38,14 +41,121 @@ module RSolvers {
     }
   }
 
-  datatype RSolver = RSolver(solver: Solvers.Solver, state: Solvers.SolverState)
+  // ===== RContext =====
+
+  trait RContext_ extends object {
+    const depth: nat
+    ghost predicate Valid()
+  }
+
+  class RContextRoot extends RContext_ {
+    ghost predicate Valid() {
+      depth == 0
+    }
+
+    constructor ()
+      ensures Valid()
+    {
+      depth := 0;
+    }
+  }
+
+  class RContextNode extends RContext_ {
+    const parent: RContext
+    const expr: RExpr
+
+    ghost predicate Valid() {
+      depth == parent.depth + 1
+    }
+
+    constructor (parent: RContext, expr: RExpr)
+      ensures Valid()
+    {
+      this.depth := parent.depth + 1;
+      this.parent := parent;
+      this.expr := expr;
+    }
+  }
+
+  type RContext = r: RContext_ | r.Valid() witness *
+
+  method CreateEmptyContext() returns (context: RContext) {
+    context := new RContextRoot();
+  }
+  
+  method Extend(context: RContext, expr: RExpr) returns (r: RContext) {
+    r := new RContextNode(context, expr);
+  }
+
+  // ===== REngine =====
+
+  class REngine {
+    const Repr: set<object>
+    ghost predicate Valid()
+      reads Repr
+      ensures Valid() ==> this in Repr
+    {
+      this in Repr
+    }
+
+    // This constructor is given a name, so that it doesn't automatically get exported just because the class is revealed
+    constructor New(state: Solvers.SolverState)
+      ensures Valid() && fresh(Repr)
+    {
+      Repr := {this};
+    }
+
+    method Prove(context: RContext, expr: RExpr)
+  }
+
+  method CreateEngine() returns (r: REngine)
+    ensures r.Valid() && fresh(r.Repr)
+  {
+    var z3 := Z3SmtSolver.CreateZ3SolverEngine();
+    var state := new Solvers.SolverState(z3);
+    r := new REngine.New(state);
+  }
+
+
+
+
+
+
+
+
+
+
+
+
+
+
+
+
+
+
+
+  method Create() returns (r: RSolver)
+    ensures r.Valid() && fresh(r.Repr)
+  {
+    var smtEngine := Z3SmtSolver.CreateZ3SolverEngine();
+    var state := new Solvers.SolverState(smtEngine);
+    var solver := Solvers.Solver.Empty();
+    return RSolver(solver, state, 0, None);
+  }
+
+  datatype RSolver = RSolver(solver: Solvers.Solver, state: Solvers.SolverState, depth: nat, previous: Option<RSolver>)
   {
     ghost const Repr: set<object> := { state, state.smtEngine, state.smtEngine.process }
 
     ghost predicate Valid()
       reads Repr
     {
-      state.Valid() && state.ValidFor(solver)
+      state.Valid() &&
+      state.ValidFor(solver) &&
+      match previous
+      case None => depth == 0
+      case Some(prev) =>
+        prev.state == state && prev.depth < depth
     }
 
     method Extend(expr: RExpr) returns (r: RSolver)
@@ -56,14 +166,15 @@ module RSolvers {
       var solver := this.solver;
       // TODO: declare the new symbols in "expr"
       solver := solver.Extend(expr.ToSExpr(), state);
-      return RSolver(solver, state);
+      r := RSolver(solver, state, depth + 1, Some(this));
     }
 
     method Prove(expr: RExpr)
       requires Valid()
       modifies Repr
       ensures Valid()
-    {      // TODO: declare the new symbols in "expr"
+    {
+      // TODO: declare the new symbols in "expr"
       solver.Prove(expr.ToSExpr(), state);
     }
 
@@ -74,7 +185,7 @@ module RSolvers {
     {
       // TODO: declare the new symbols in "expr"
       var solver := solver.Record(expr.ToSExpr());
-      return RSolver(solver, state);
+      return RSolver(solver, state, depth + 1, Some(this));
     }
   }
 }
